libcrux-ml-kem/proofs/fstar/extraction/Libcrux_ml_kem.Vector.Avx2.Arithmetic.fsti
@@ -87,12 +87,11 @@ val montgomery_multiply_by_constant
       (vector: Libcrux_intrinsics.Avx2_extract.t_Vec256)
       (constant: i16)
     : Prims.Pure Libcrux_intrinsics.Avx2_extract.t_Vec256
-      (requires Spec.Utils.is_i16b 3328 constant)
+      (requires Spec.Utils.is_i16b 1664 constant)
       (ensures
         fun result ->
           let result:Libcrux_intrinsics.Avx2_extract.t_Vec256 = result in
-          Spec.Utils.is_i16b_array (3328 + 1665)
-            (Libcrux_intrinsics.Avx2_extract.vec256_as_i16x16 result) /\
+          Spec.Utils.is_i16b_array 3328 (Libcrux_intrinsics.Avx2_extract.vec256_as_i16x16 result) /\
           (forall i.
               i < 16 ==>
               v (get_lane result i) % 3329 == ((v (get_lane vector i) * v constant * 169) % 3329)))
@@ -100,12 +99,11 @@ val montgomery_multiply_by_constant
 val montgomery_multiply_by_constants (vec constants: Libcrux_intrinsics.Avx2_extract.t_Vec256)
     : Prims.Pure Libcrux_intrinsics.Avx2_extract.t_Vec256
       (requires
-        Spec.Utils.is_i16b_array 3328 (Libcrux_intrinsics.Avx2_extract.vec256_as_i16x16 constants))
+        Spec.Utils.is_i16b_array 1664 (Libcrux_intrinsics.Avx2_extract.vec256_as_i16x16 constants))
       (ensures
         fun result ->
           let result:Libcrux_intrinsics.Avx2_extract.t_Vec256 = result in
-          Spec.Utils.is_i16b_array (3328 + 1665)
-            (Libcrux_intrinsics.Avx2_extract.vec256_as_i16x16 result) /\
+          Spec.Utils.is_i16b_array 3328 (Libcrux_intrinsics.Avx2_extract.vec256_as_i16x16 result) /\
           (forall i.
               i < 16 ==>
               v (get_lane result i) % 3329 ==
@@ -114,12 +112,11 @@ val montgomery_multiply_by_constants (vec constants: Libcrux_intrinsics.Avx2_ext
 val montgomery_multiply_m128i_by_constants (vec constants: Libcrux_intrinsics.Avx2_extract.t_Vec128)
     : Prims.Pure Libcrux_intrinsics.Avx2_extract.t_Vec128
       (requires
-        Spec.Utils.is_i16b_array 3328 (Libcrux_intrinsics.Avx2_extract.vec128_as_i16x8 constants))
+        Spec.Utils.is_i16b_array 1664 (Libcrux_intrinsics.Avx2_extract.vec128_as_i16x8 constants))
       (ensures
         fun result ->
           let result:Libcrux_intrinsics.Avx2_extract.t_Vec128 = result in
-          Spec.Utils.is_i16b_array (3328 + 1665)
-            (Libcrux_intrinsics.Avx2_extract.vec128_as_i16x8 result) /\
+          Spec.Utils.is_i16b_array 3328 (Libcrux_intrinsics.Avx2_extract.vec128_as_i16x8 result) /\
           (forall i.
               i < 8 ==>
               v (get_lane128 result i) % 3329 ==
@@ -135,7 +132,7 @@ val montgomery_reduce_i32s (vec: Libcrux_intrinsics.Avx2_extract.t_Vec256)
           let result:Libcrux_intrinsics.Avx2_extract.t_Vec256 = result in
           Spec.Utils.is_i16b_array (3328 + 1665)
             (Libcrux_intrinsics.Avx2_extract.vec256_as_i16x16 result) /\
-          (Spec.Utils.is_i16b_array (3328 * 3328)
+          (Spec.Utils.is_i16b_array (3328 * pow2 15)
               (Libcrux_intrinsics.Avx2_extract.vec256_as_i16x16 vec) ==>
             Spec.Utils.is_i16b_array 3328 (Libcrux_intrinsics.Avx2_extract.vec256_as_i16x16 result)) /\
           (forall i. i < 16 ==> v (get_lane result i) % 3329 == ((v (get_lane vec i) * 169) % 3329))
